eccentricity
- e=0 - circle
- 0<e<1 - ellipse
- e=1 - parabola
- e>1 - Hyperbola

Infinite series
- $e^x=1+x+\frac{x^2}{2!}+...$

# Derivations
- ${\frac{d}{d x}}\left(e^{a x}\right)=a e^{a x}$
- ${\frac{d}{d x}}(\ln a x)={\frac{1}{x}}$
- ${\frac{d}{d x}}\left(\sin^{-1}{\frac{x}{a}}\right)={\frac{1}{\sqrt{a^{2}-x^{2}}}}$
- $\frac{d}{d x}\left(\cos^{-1}\frac{x}{a}\right)=\frac{-1}{\sqrt{a^{2}-x^{2}}},\quad\frac{d}{d x}\left(\tan^{-1}\frac{x}{a}\right)=\frac{a}{a^{2}+x^{2}}$
- $(uvw)^{\prime}=uvw^{\prime}+uv^{\prime}w+u^{\prime}v w$

### Leibinitz theorm
$f^{(n)}=\sum_{r=0}^{n}\frac{n!}{r!(n-r)!}u^{(r)}v^{(n-r)}=\sum_{r=0}^{n}\ ^{n}C_{r}u^{(r)}v^{(n-r)}$


- radius of curvature $\rho={\frac{\left[1+(f^{\prime})^{2}\right]^{3/2}}{f^{\prime\prime}}}$

- Lagrange multipliers 
	If $f$ is the function to be maximized and the function $\phi$ describes a relation between the variables $F(x,y,z)=f+\lambda\phi$
# Vector 
- Lagrange's identity $(\mathbf{a}\times\mathbf{b})\cdot(\mathbf{c}\times\mathbf{d})\equiv(\mathbf{a}\cdot\mathbf{c})(\mathbf{b}\cdot\mathbf{d})-(\mathbf{a}\cdot\mathbf{d})(\mathbf{b}\cdot\mathbf{c})$
### scalar triple product 
$\mathbf{a},\mathbf{b},\mathbf{c}\ =\left[\mathbf{b},\mathbf{c},\mathbf{a}\right]=\left[\mathbf{c},\mathbf{a},\mathbf{b}\right]=-\left[\mathbf{a},\mathbf{c},\mathbf{b}\right]=-\left[\mathbf{b},\mathbf{a},\mathbf{c}\right]=-\left[\mathbf{c},\mathbf{b},\mathbf{a}\right]$
### Vector triple product
-  $a\times b \times c =b(a\cdot c)-c(a \cdot b)$
- $\mathbf{a}\times(\mathbf{b}\times\mathbf{c})+\mathbf{b}\times(\mathbf{c}\times\mathbf{a})+\mathbf{c}\times(\mathbf{a}\times\mathbf{b})=\mathbf{0}$

# Polar Coordinate
$x=r\cos\theta$
$y=r\sin\theta$
$z= z$
$r=\sqrt{x^2+y^2}$
$\theta = \tan^{-1} (\frac{y}{x})$
- $\hat{r}(\theta)=\cos\theta\hat{x}+\sin\theta\hat{y}$
- $\hat{\theta}(\theta)=-\sin\theta\hat{x}+\cos\theta\hat{y}$

- ${\frac{d{\hat{\mathbf{r}}}}{d t}}={\dot{\theta}}{\hat{\boldsymbol{\theta}}}$
- $\frac{d\hat{\theta}}{d t}=-\dot{\theta}\hat{\mathrm{r}}$

- $\mathbf{v}={\frac{d}{d t}}(r{\hat{\mathbf{r}}})=\dot{r}\hat{r}+r\dot{\theta}\hat{\theta}$
- $\mathbf{a}=\left({\ddot{r}}-r{\dot{\theta}}^{2}\right){\hat{\mathbf{r}}}+(r{\ddot{\theta}}+2{\dot{r}}{\dot{\theta}}){\hat{\boldsymbol{\theta}}}$
	- $a=a_R \hat{r}+a_T \hat{\theta}$




